lakefile.lean
@@ -11,5 +11,6 @@ require verity from git
 lean_lib «Benchmark» where
   globs := #[
     .one `Benchmark,
-    .andSubmodules `Benchmark.Cases
+    .andSubmodules `Benchmark.Cases,
+    .andSubmodules `Benchmark.Generated.NexusMutual
   ]
